lib/Behaviors.v
@@ -15,7 +15,7 @@
 
 (** Whole-program behaviors *)
 
-Require Import Parameters.
+Require Import UNIVERSE.
 Require Import Classical.
 Require Import ClassicalEpsilon.
 Require Import Coqlib.
