lib/Smallstep.v
@@ -20,7 +20,7 @@
   operational semantics in small-step style. *)
 
 
-Require Import Parameters.
+Require Import UNIVERSE.
 
 Require Import Relations.
 Require Import Wellfounded.
