lib/SmallstepC.v
@@ -1,4 +1,4 @@
-Require Import Parameters.
+Require Import UNIVERSE.
 Require Import Relations.
 Require Import Wellfounded.
 Require Import CoqlibC.
