proof/AdequacySound.v
@@ -1,4 +1,4 @@
-Require Import Parameters.
+Require Import UNIVERSE.
 Require Import CoqlibC.
 Require Import Simulation.
 Require Import LinkingC.
