proof/ModSemProps.v
@@ -1,4 +1,4 @@
-Require Import Parameters.
+Require Import UNIVERSE.
 (* Require Import EventsC. *)
 (* Require Import Values. *)
 (* Require Import AST. *)
